\documentclass[12pt, border = 4pt, multi]{article} % \documentclass[tikz, border = 4pt, multi]{article}
\usepackage[a4paper, margin = 70pt]{geometry}
\usepackage{lingmacros}
\usepackage{tree-dvips}
\usepackage{amssymb} % mathbb{}
\usepackage[dvipsnames]{xcolor}
\usepackage{forest}
\usepackage[pdftex]{hyperref}
\usepackage{amsmath} % matrices
\usepackage{xeCJK}
\usepackage{tikz}
\usepackage[arrowdel]{physics}
\usepackage{graphicx}
\usepackage{wrapfig}
\usepackage{listings}
\usepackage{pgfplots, pgfplotstable}
\usepackage{diagbox} % diagonal line in cell
\usepackage[usestackEOL]{stackengine}
\usepackage{makecell}
\usepackage{multirow}
\usepackage{multicol}
\usepackage[T1]{fontenc} 
\setlength{\columnsep}{1cm}
\graphicspath{{./img}} % specify the graphics path to be relative to the main .tex file, denoting the main .tex file directory as ./
\definecolor{orchid}{rgb}{0.7, 0.4, 1.1}
\lstset
{ 
  backgroundcolor = \color{white},
  basicstyle = \scriptsize,
  breaklines = true,
  commentstyle = \color{comment_color}\textit,
  keywordstyle = \color{keyword_color}\bfseries,
  language = c++,
  escapeinside = {\%*}{*)},          
  extendedchars = true,              
  frame = tb,
  numberstyle = \tiny\color{comment_color},
  rulecolor = \color{black},
  showstringspaces = false,
  stringstyle = \color{string_color},
  upquote = true, 
}
\usepackage{xcolor}
\definecolor{comment_color}{rgb}{0, 0.5, 0}
\definecolor{keyword_color}{rgb}{0.3, 0, 0.6}
\definecolor{string_color}{rgb}{0.5, 0, 0.1}
\begin{document}
\section*{Xi Liu}
1.\\
power set is set of all subsets of $X$\\
$\mathcal{P}(X) = \{S: S \subset X\}$\\
$C$ is an upper bound of $A$: $\forall B \in A, B \subset C$\\
$S$ is an least upper bound of $A$: $\forall \text{ upper bounds } C \text{ of } A, S \subset C$\\
\\
(a)\\
$C := B_1 \cup B_2$ is an upper bound of $A := \{B_1, B_2\}$\\
need to show $\forall B \in A := \{B_1, B_2\}, B \subset C := B_1 \cup B_2$\\
if $B = B_1, \forall x (x \in B_1 \rightarrow x \in B_1 \vee x \in B_2), B_1 \subset B_1 \cup B_2$\\
if $B = B_2, \forall x (x \in B_2 \rightarrow x \in B_1 \vee x \in B_2), B_2 \subset B_1 \cup B_2$\\
\\
\\
(b)\\
part 1\\
if $C$ is an upper bound of $A := \{B_1, B_2\}$\\
then $\forall B \in A := \{B_1, B_2\}, B \subset C$\\
$\because B_1 \subset C, \forall x(x \in B_1 \rightarrow x \in C)\\
B_2 \subset C, \forall x(x \in B_2 \rightarrow x \in C)\\
\therefore \forall x(x \in B_1 \vee x \in B_2 \rightarrow x \in C), B_1 \cup B_2 \subset C\\$
\\
part 2\\
$B_1 \cup B_2$ is a least upper bound: since $\forall$ upper bounds $C$ of $A := \{B_1, B_2\}$, $B_1 \cup B_2 \subset C$ as shown in part 1\\
if $S$ is another least upper bound, then\\
(i) $S$ is an upper bound of $A$, $\forall B \in A, B \subset S, \forall x (x \in B \rightarrow x \in S)$\\
(ii) $S$ is a least upper bound of $A$, $\forall$ upper bounds $C$ of $A := \{B_1, B_2\}$, $S \subset C, \forall x (x \in S \rightarrow x \in C)$\\
\\
$\because S$ is an upper bound, and $B_1 \cup B_2$ is the least upper bound\\
$\therefore B_1 \cup B_2 \subset S$\\
\\
$\because B_1 \cup B_2$ is an upper bound\\
$\therefore S \subset B_1 \cup B_2$\\
\\
$\because B_1 \cup B_2 \subset S, S \subset B_1 \cup B_2\\
\therefore S = B_1 \cup B_2$\\
\\
\\
(c)\\
$C$ is an lower bound of $A$: $\forall B \in A, C \subset B$\\
$B_1 \cap B_2$ is a lower bound of $\{B_1, B_2\}$\\
need to show $\forall B \in A := \{B_1, B_2\}, C :=  B_1 \cap B_2 \subset B$\\
if $B = B_1, \forall x (x \in B_1 \wedge x \in B_2 \rightarrow x \in B_1), B_1 \cap B_2 \subset B_1$\\
if $B = B_2, \forall x (x \in B_1 \wedge x \in B_2 \rightarrow x \in B_2), B_1 \cap B_2 \subset B_2$\\
\\
\\
(d)\\
show every nonempty collection $A \subset \mathcal{P}(X)$ has a least upper bound $S$\\
since $A$ is nonempty, exists a set $\bigcup_{B \in A} B$ which is the union over this collection
\[\bigcup_{B \in A} B := \{x \in X: \exists B \in A, x \in B\}\]
$\forall B \in A, \forall x(x \in B \rightarrow x \in \bigcup_{B \in A} B), B \subset \bigcup_{B \in A} B$, so $\bigcup_{B \in A} B$ is an upper bound\\
since $S := \bigcup_{B \in A} B$ is the union of all sets in $A$, $S := \bigcup_{B \in A} B$ contains all elements of all sets in $A$ and no extra element, so it has the least cardinality among all upper bounds of $A$, $\forall$ upper bounds $C$ of $A$, $S \subset C$, so $S := \bigcup_{B \in A} B$ is the least upper bound of $A$\\
\\
\\
2.\\
(a)\\
let $a := \sup S$, since $a$ is an least upper bound, $a - 1$ is not an upper bound of $S$, so $\exists x_1 \in S, a - 1 \leq x_1 \leq a$\\
continuing, construct a monotone increasing sequence $x_n, \forall n \in \mathbb{N}, a - 1 / n < x_n \leq a$, since $\lim_{n \rightarrow \infty} a - 1 / n = a$ and $\lim_{n \rightarrow \infty} a = a$, by squeeze lemma, $x_n$ converges to $a$\\
\\
\\
(b)\\
base step: $\{y_n\} = \{y_1\} \in S$, monotone increasing\\
inductive step: assume $y_1, ..., y_n = \{y_n\} \in S$ is monotone increasing, need to show $y_1, ..., y_{n + 1} = \{y_{n + 1}\} \in S$ is also monotone increasing\\
$\because \sup S \not\in S, \forall n \in \mathbb{N}, \forall y_n \in S, y_n < \sup S \\
\sup S - y_n > 0\\
\text{base on hw1 q8}, \forall \varepsilon > 0, \exists x \in B, c - \varepsilon < x \leq c\\
\exists y_{n + 1} \in S, y_n < y_{n + 1} < \sup S$\\
so $\{y_{n + 1}\}$ is shown to be monotone increasing\\
$\{y_n\}$ is a monotone increasing sequence\\
\\
\\
(c)\\
since there exists a strictly monotone increasing sequence $\{y_n\}$ with $y_n \in S, \forall n \in \mathbb{N}$, establish a bijective function $f: \{y_n : n \in \mathbb{N}\} \rightarrow \mathbb{N}, f(y_n) = n$\\
\\
\\
(d)\\
let $S$ be the empty set, $S = \emptyset \subset \mathbb{R}$, then $S$ only have 1 subset $E = \emptyset$ that is itself, $\emptyset$ is finite so it is not countably infinite\\
so not always be a countably infinite subset\\
\\
\\
3.\\
(a)\\
part 1\\
$\{x_n\}$ diverges to negative infinity: $\forall K \in \mathbb{R}, \exists M \in \mathbb{N}, \forall n \geq M, x_n \leq -k, \lim_{n \rightarrow \infty} x_n := -\infty$\\
part 2\\
$\{x_n\} := \{-n ^ 3\}, M := \sqrt[3]{K}\\
\forall K \in \mathbb{R}, \forall n \geq M, -n \leq -M, x_n = -n ^ 3 \leq -M ^ 3 = -(\sqrt[3]{K}) ^ 3 = -K\\
x_n \leq -K$, $x_n$ diverges to $-\infty$\\
\\
\\
(b)\\
\begin{align*}
\lim_{n \rightarrow \infty} \frac{1}{x_n} &= 0\\
\forall K_1 \geq 0, \exists M \in \mathbb{N}, &\forall n \geq M\\
\left|\frac{1}{x_n} - 0\right| &< K_1\\
1 &< K_1 x_n\\
x_n &> \frac{1}{K_1}\\
K_2 &:= \frac{1}{K_1}\\
x_n &> K_2
\end{align*}
so $\{x_n\}$ diverges to positive infinity\\
\\
\\
(c)\\
definition 1.3.6\\
$f: D \rightarrow \mathbb{R}$\\
$f$ is bounded: $\exists M \in \mathbb{R}, \forall x \in D, |f(x)| \leq M$\\
$f$ is unbounded: $\forall M \in \mathbb{R}, \exists x \in D, |f(x)| > M$\\
$f$ is unbounded above: $\forall M \in \mathbb{R}, \exists x \in D, f(x) > M$\\
\\
part 1\\
if $\{x_n\}$ is unbounded above, then $\{x_n\}$ has a subsequence $\{x_{n_k}\}$ that diverges to positive infinity\\
(i) if $\{x_n\}$ is unbounded above, then every $p$-tail of $\{x_n\}$ is also unbounded above\\
if $\{x_n\}$ is unbounded above\\
base step: since $\{x_n\}_{n = 1} ^ {\infty}$ is unbounded above,  based on definition of unbounded above, $\forall k \in \mathbb{R}, \exists n \in \mathbb{N}, f(n) := x_n > k$, so choose $k = 1$, $\exists n_1 \in \mathbb{N}, x_{n_1} > 1$, $n_1$-tail of $x_n$ starts with the term after $x_{n_1}, n_1 < n_2$, if choose $k = 2$, $\exists n_2 \in \mathbb{N}, x_{n_2} > 2$\\
inductive step: suppose $x_{n_p}$ is defined for some $p$, need to define $x_{n_{p + 1}}$, based on definition of unbounded above, $\forall k \in \mathbb{R}, \exists n \in \mathbb{N}, f(n) := x_n > k, \text{so }\exists n_p \in \mathbb{N}, f(n_p) := x_{n_p} > p$, $n_p$-tail is the sequence $\{x_{i + n_p}\}_{i = 1} ^ {\infty}$ starting at index $n_p + 1$, $n_{p + 1}$-tail is the sequence $\{x_{i + n_{p + 1}}\}_{i = 1} ^ {\infty}$ starting at index $n_{p + 1} + 1$, since $n_p$-tail of $x_n$ starts with the term after $x_{n_p}, n_p < n_{p + 1}$, $n_{p + 1}$-tail is defined, based on definition of unbounded above, $k = p + 1$, $\exists n_{p + 1} \in \mathbb{N}, x_{n_{p + 1}} > p + 1$\\
so $\forall k \in \mathbb{R}, \exists M \in \mathbb{N}, \forall n \geq M, x_{n_k} > k$\\
\\
part 2\\
if $\{x_n\}$ has a subsequence $\{x_{n_k}\}$ that diverges to positive infinity, then $\{x_n\}$ is unbounded above\\
if $\{x_n\}$ has a subsequence $\{x_{n_k}\}$ that diverges to positive infinity, then\\ $\forall K \in \mathbb{R}, \exists M \in \mathbb{N}, \forall n \geq M, x_{n_k} > K$\\
let $x_{n_k} := x_k := k$, for contradiction, assume $\{x_n\}$ is bounded above, let $b := \sup\{x_n\}$, number $b - 1$ cannot be an upper bound for $\{x_n\}$ as it is strictly less than $b$ (the least upper bound). $\exists m \in \mathbb{N}, m > b - 1, m + 1 = x_m + 1 > b$, contradicting $b$ being an upper bound, so $\{x_n\}$ is unbounded above\\
\\
\\
\\
4.\\
(a)
\begin{align*}
\text{if } n \text{ is even, then }\\
\{\bar{x}_n\} = \frac{1}{n}\sum_{i = 1} ^ n (-1) ^ n &= 0\\
\text{if } n \text{ is odd, then }\\
\{\bar{x}_n\} = \frac{1}{n}\sum_{i = 1} ^ n (-1) ^ n &= -\frac{1}{n}\\ 
\end{align*}
if $n$ is even, then\\
$\forall \varepsilon > 0, \exists M \in \mathbb{N}, \forall n \geq M, |\bar{x}_n - 0| = |0 - 0| = 0 < \varepsilon$\\
if $n$ is odd, then\\
$\forall \varepsilon > 0, \exists M \in \mathbb{N}, 0 < 1 / M < \varepsilon, \forall n \geq M, |\bar{x}_n - 0| = |-1 / n - 0| = 1 / n \leq 1 / M < \varepsilon$\\
\\
\\
(b)
\begin{align*}
|\bar{x}_n - L| &= \left|\left(\frac{1}{n}\sum_{k = 1} ^ n x_k\right) - L\right|\\
&= \left|\left(\frac{1}{n}\sum_{k = 1} ^ n x_k\right) - \frac{nL}{n}\right|\\
&= \left|\sum_{k = 1} ^ n\frac{x_k - L}{n}\right|\\
&= \left|\sum_{k = 1} ^ M\frac{x_k - L}{n} + \sum_{k = M + 1} ^ n\frac{x_k - L}{n}\right|\\
&= \left|\frac{1}{n}\sum_{k = 1} ^ M x_k - L + \frac{1}{n}\sum_{k = M + 1} ^ n x_k - L\right|\\
&\leq \frac{1}{n}\sum_{k = 1} ^ M |x_k - L| + \frac{1}{n}\sum_{k = M + 1} ^ n |x_k - L|\\
&\text{/* since } |x_n - L| < \varepsilon / 2 \text{ */}\\
&< \frac{1}{n}\sum_{k = 1} ^ M \left(\frac{\varepsilon}{2}\right) + \frac{1}{n}\sum_{k = M + 1} ^ n \left(\frac{\varepsilon}{2}\right)\\
&= \frac{(M - 1 + 1)}{n}\frac{\varepsilon}{2} + \frac{n - (M + 1) + 1}{n}\frac{\varepsilon}{2}\\
&= \frac{M\varepsilon}{2n} + \frac{(n - M)\varepsilon}{2n}\\
&\text{/* since } \exists K \geq \frac{\varepsilon}{2} \text{ */}\\
&\leq \frac{MK}{n} + \frac{(n - M)\varepsilon}{2n}\\
\end{align*}
\\
\\
(c)
\begin{align*}
\frac{MK}{n} + \frac{(n - M)\varepsilon}{2n} &\leq \frac{MK}{n} + \frac{n\varepsilon}{2n}\\
&= \frac{MK}{n} + \frac{\varepsilon}{2}\\
&\text{/* }\forall n > \frac{2MK}{\varepsilon}\text{ */}\\
&< \frac{MK}{2MK / \varepsilon} + \frac{\varepsilon}{2}\\
&= \frac{\varepsilon}{2} + \frac{\varepsilon}{2}\\
&= \varepsilon
\end{align*}
since $MK / n$ converges to 0
\begin{align*}
&\text{show } \frac{MK}{n} \text{ converges to 0}\\
&\forall \varepsilon > 0, \exists m \in \mathbb{N}, 0 < MK / m < \varepsilon, \forall n \geq m\\
&\left|\frac{MK}{n} - 0\right| = MK / n \leq MK / m < \varepsilon
\end{align*}
\end{document}
