\documentclass[12pt, border = 4pt, multi]{article} % \documentclass[tikz, border = 4pt, multi]{article}
\usepackage[a4paper, margin = 70pt]{geometry}
\usepackage{lingmacros}
\usepackage{tree-dvips}
\usepackage{amssymb} % mathbb{}
\usepackage[dvipsnames]{xcolor}
\usepackage{forest}
\usepackage[pdftex]{hyperref}
\usepackage{amsmath} % matrices
\usepackage{xeCJK}
\usepackage{tikz}
\usepackage[arrowdel]{physics}
\usepackage{graphicx}
\usepackage{wrapfig}
\usepackage{listings}
\usepackage{pgfplots, pgfplotstable}
\usepackage{diagbox} % diagonal line in cell
\usepackage[usestackEOL]{stackengine}
\usepackage{makecell}
\usepackage{multirow}
\usepackage{multicol}
\usepackage[T1]{fontenc} 
\setlength{\columnsep}{1cm}
\graphicspath{{./img}} % specify the graphics path to be relative to the main .tex file, denoting the main .tex file directory as ./
\definecolor{orchid}{rgb}{0.7, 0.4, 1.1}
\lstset
{ 
  backgroundcolor = \color{white},
  basicstyle = \scriptsize,
  breaklines = true,
  commentstyle = \color{comment_color}\textit,
  keywordstyle = \color{keyword_color}\bfseries,
  language = c++,
  escapeinside = {\%*}{*)},          
  extendedchars = true,              
  frame = tb,
  numberstyle = \tiny\color{comment_color},
  rulecolor = \color{black},
  showstringspaces = false,
  stringstyle = \color{string_color},
  upquote = true, 
}
\usepackage{xcolor}
\definecolor{comment_color}{rgb}{0, 0.5, 0}
\definecolor{keyword_color}{rgb}{0.3, 0, 0.6}
\definecolor{string_color}{rgb}{0.5, 0, 0.1}
\begin{document}
\section*{Xi Liu}
collaboration: Chuanyang Jin\\
\\
1.\\
(i)\\
subset definition
\begin{align*}
S_1 \subset S_2 &\equiv \forall x (x \in S_1 \rightarrow x \in S_2) \qquad (*)\\
S_1 \subset S_2 &\equiv S_2 \supset S_1
\end{align*}
prove if $C \subset B$ and $B \subset A$, then $C \subset A$
\begin{align*}
&\forall c \in C, \quad\because C \subset B, \quad\therefore c \in B \qquad (*)\\
&\because B \subset A, \quad \quad\therefore c \in A \qquad (*)
\end{align*}
so it is shown $\forall c(c \in C \rightarrow c \in A) \equiv C \subset A$\\
\\
\\
(ii)\\
set equality definition
\begin{align*}
S_1 &= S_2 \equiv (S_1 \subset S_2) \wedge (S_2 \subset S_1) \equiv \forall x (x \in S_1 \leftrightarrow x \in S_2) \qquad (*)\\
&\text{prove } (S_1 \subset S_2) \wedge (S_2 \subset S_1)\\
&A \subset C:\\
&\forall a \in A, \quad\because A = B, \quad\therefore a \in B\\
&\because B = C, \quad\therefore a \in C\\
&\text{so it is shown } \forall a (a \in A \rightarrow a \in C) \equiv A \subset C\\
&C \subset A:\\
&\forall c \in C, \quad\because B = C, \qquad\therefore c \in B\\
&\because A = B, \quad\therefore c \in A\\
&\text{so it is shown } \forall c (c \in C \rightarrow c \in A) \equiv C \subset A\\
&\text{so it is shown } (A \subset C) \wedge (C \subset A) \equiv \forall x (x \in A \leftrightarrow x \in C) \equiv A \equiv C\\
\end{align*}
\\
\\
\\
2.\\
(a)
\begin{align*}
&\forall x_1, x_2 \in (0, 1), \text{if } f(x_1) = \frac{1}{x_1}, f(x_2) = \frac{1}{x_2}, \text{and } f(x_1) =f(x_2),\\
&\text{then } \frac{1}{x_1} = \frac{1}{x_2}\\
&\frac{1}{1 / x_1} = \frac{1}{1 / x_2}\\
&x_1 = x_2\\
&\text{so it is shown } \forall x_1, x_2 \in (0, 1), f(x_1) = f(x_2) \rightarrow x_1 = x_2
\end{align*}
so $f$ is injective
\begin{align*}
\forall f(x) &\in (1, \infty)\\
f(x) &= \frac{1}{x}\\
x &= \frac{1}{f(x)}\\
\because f(x) &\in (1, \infty)\\
\therefore x &= \frac{1}{f(x)} < 1\\
\because f(x) \geq 1 > 0 &\text{ and } 1 > 0\\
\therefore x &= \frac{1}{f(x)} > 0\\
0 &< \frac{1}{f(x)} < 1\\
0 &< x < 1
\end{align*}
so it is shown $\forall f(x) \in (1, \infty), \exists x \in (0, 1)$ such that $f(x) = 1 / x$\\
so $f$ is surjective\\
\\
(b)\\
\begin{align*}
&\text{let } x_1 = 1.0 \in \mathbb{R}, x_2 = 1.1 \in \mathbb{R}\\
&g(x_1) = g(1.0) = \lfloor 1.0 \rfloor = 1\\
&g(x_2) = g(1.1) = \lfloor 1.1 \rfloor = 1\\
&g(x_1) = 1 = g(x_2) \text{ but } x_1 = 1.0 \not= 1.1 = x_2
\end{align*}
so $g$ is not injective\\
\\
$\forall z \in \mathbb{Z}$, since $z$ is an integer, floor of $z$ is equal to $z$ itself, so $\forall z \in \mathbb{Z}, \exists z \in \mathbb{R}, g(z) = \lfloor z \rfloor = z$, so $g$ is surjective\\
\\
\\
\\
3.\\
(a)\\
bijective is both injective and surjective\\
show $f_3$ is injective\\
$\forall \textbf{v}_1, \textbf{v}_2 \in \mathbb{N} ^ 3$, denote $\textbf{v}_1 = (\textbf{v}_1.x, \textbf{v}_1.y, \textbf{v}_1.z), \quad\textbf{v}_2 = (\textbf{v}_2.x, \textbf{v}_2.y, \textbf{v}_2.z)$,\\
if $f_3(\textbf{v}_1) = f_3(\textbf{v}_2)$,\\
then $(\textbf{v}_1.x, f_2(\textbf{v}_1.y, \textbf{v}_1.z)) = (\textbf{v}_2.x, f_2(\textbf{v}_2.y, \textbf{v}_2.z))$,\\
then $\textbf{v}_1.x = \textbf{v}_2.x$ and $f_2(\textbf{v}_1.y, \textbf{v}_1.z) = f_2(\textbf{v}_2.y, \textbf{v}_2.z)$\\
$f_2$ is defined to be a bijective function as stated, where the elements in $\mathbb{N} \times \mathbb{N}$ are arranged by in increasing order according to the sum of 2 entries ($(1, 1), (1, 2), (2, 1), (1, 3), ...$), and assign $f_2(1, 1) = 1, f_2(1, 2) = 2, f_2(2, 1) = 3, ...$\\
$\because f_2$ is bijective, $\therefore f_2$ is injective, and since we know $f_2(\textbf{v}_1.y, \textbf{v}_1.z) = f_2(\textbf{v}_2.y, \textbf{v}_2.z)$ and $f_2$ is injective, so $(\textbf{v}_1.y, \textbf{v}_1.z) = (\textbf{v}_2.y, \textbf{v}_2.z)$,\\
so $\textbf{v}_1 = (\textbf{v}_1.x, \textbf{v}_1.y, \textbf{v}_1.z) = (\textbf{v}_2.x, \textbf{v}_2.y, \textbf{v}_2.z) = \textbf{v}_2$,\\
so $f_3$ is injective\\
\\
show $f_3$ is surjective\\
$\forall \textbf{y} \in \mathbb{N} ^ 2$, denote $\textbf{y} = (\textbf{y}.x, \textbf{y}.y),\\
\text{show }\forall \textbf{y} \in \mathbb{N} ^ 2, \exists \textbf{x} = (n_1, n_2, n_3)\in \mathbb{N} ^ 3, f(\textbf{x}) = \textbf{y}\\
\forall (n_1, f_2(n_2, n_3)) \in \mathbb{N} ^ 2$, since $\textbf{y}.x = n_1 = \textbf{x}.x$, so $n_1$ exists,\\
since $f_2$ is defined to be a surjective function as stated, $\forall \textbf{y}_2 \in \mathbb{N}, \exists \textbf{x}_2 = (n_2, n_3) \in \mathbb{N} ^ 2$ such that $f_2(\textbf{x}_2) = f_2(n_2, n_3) = \textbf{y}_2$, so $n_2, n_3$ exist\\
since $n_1, n_2, n_3$ exist, $\text{it is shown that }\forall \textbf{y} \in \mathbb{N} ^ 2, \exists \textbf{x} \in \mathbb{N} ^ 3, f(\textbf{x}) = \textbf{y}$\\
so $f_3$ is surjective\\
\\
(b)\\
let $prop(p)$ be the proposition that $\mathbb{N} ^ p$ is countable\\
\\
base step: if $p = 1$, $f_1: \mathbb{N} \rightarrow \mathbb{N}$, establish a bijection by choosing $f_1(n) = n$, then $\forall n_1, n_2 \in \mathbb{N}, f_1(n_1) = f_2(n_2) \rightarrow n_1 = n_2, \text{ and }\forall y = f_1(n) \in \mathbb{N}, \exists n \in \mathbb{N} \text{ such that } f_1(n) = n = y$, so $|\mathbb{N}| = |\mathbb{N}|$, so based on definition of countable, $\mathbb{N}$ is countable\\
if $p = 2$, $f_2$ is defined to be a bijective function as stated, where the elements in $\mathbb{N} \times \mathbb{N}$ are arranged by in increasing order according to the sum of 2 entries ($(1, 1), (1, 2), (2, 1), (1, 3), ...$), and assign $f_2(1, 1) = 1, f_2(1, 2) = 2, f_2(2, 1) = 3, ...$, so $|\mathbb{N} ^ 2| = |\mathbb{N}|$, so based on definition of countable, $\mathbb{N} ^ 2$ is countable\\
if $p = 3$, it is shown in problem 3 part (a)\\
\\
inductive step: assume $i \in \mathbb{N}, prop(i)$ is true, need to show $prop(i + 1)$ is true\\
since $prop(i)$ is assumed to be true, there is a bijection $f_i: \mathbb{N} ^ i \rightarrow \mathbb{N} ^ {i - 1}$,\\
need to show there is a bijection $f_{i + 1}: \mathbb{N} ^ {i + 1} \rightarrow \mathbb{N} ^ i \text{ by } f_{i + 1}(n_1, n_2, ..., n_{i + 1}) := (n_1, f_i(n_2, n_3, ..., n_{i + 1}))$\\
denote $\textbf{v} = (\textbf{v}[1], \textbf{v}[2], ..., \textbf{v}[i + 1]) \in \mathbb{N} ^ {i + 1}$\\
\\
show $f_{i + 1}$ is injective\\
$\forall \textbf{v}_1, \textbf{v}_2 \in \mathbb{N} ^ {i + 1}, \text{ if } f(\textbf{v}_1) = f(\textbf{v}_2)$,\\
then $(\textbf{v}_1[1], f_i(\textbf{v}_1[2], \textbf{v}_1[3], ..., \textbf{v}_1[i + 1])) = (\textbf{v}_2[1], f_i(\textbf{v}_2[2], \textbf{v}_2[3], ..., \textbf{v}_2[i + 1]))$,\\
then $\textbf{v}_1[1] = \textbf{v}_2[1]$ and $f_i(\textbf{v}_1[2], \textbf{v}_1[3], ..., \textbf{v}_1[i + 1]) = f_i(\textbf{v}_2[2], \textbf{v}_2[3], ..., \textbf{v}_2[i + 1])$\\
since $f_i$ is assumed to be bijective (so injective) in the inductive hypothesis, knowing $f_i(\textbf{v}_1[2], \textbf{v}_1[3], ..., \textbf{v}_1[i + 1]) = f_i(\textbf{v}_2[2], \textbf{v}_2[3], ..., \textbf{v}_2[i + 1])$ implies $(\textbf{v}_1[2], \textbf{v}_1[3], ..., \textbf{v}_1[i + 1]) = (\textbf{v}_2[2], \textbf{v}_2[3], ..., \textbf{v}_2[i + 1])$\\
so $\textbf{v}_1 = (\textbf{v}_1[1], \textbf{v}_1[2], ..., \textbf{v}_1[i + 1]) = (\textbf{v}_2[1], \textbf{v}_2[2], ..., \textbf{v}_2[i + 1]) = \textbf{v}_2$\\
so $f_{i + 1}$ is injective\\
\\
show $f_{i + 1}$ is surjective\\
$\forall \textbf{y} \in \mathbb{N} ^ i$, denote $\textbf{y} = (\textbf{y}[1], \textbf{y}[2], ..., \textbf{y}[i]),\\
\text{show }\forall \textbf{y} \in \mathbb{N} ^ i, \exists \textbf{x} = (\textbf{x}[1], \textbf{x}[2], ..., \textbf{x}[i + 1]) = (n_1, n_2, ..., n_{i + 1})\in \mathbb{N} ^ {i + 1}, f(\textbf{x}) = \textbf{y}\\
\forall (n_1, f_i(n_2, n_3, ..., n_i)) \in \mathbb{N} ^ i$, since $\textbf{y}[1] = n_1 = \textbf{x}[1]$, so $n_1$ exists,\\
since $f_i$ is assumed to be a bijective (so surjective) function in the inductive hypothesis, $\forall \textbf{y}_2 \in \mathbb{N} ^ {i - 1}, \exists \textbf{x}_2 = (n_2, n_3, ..., n_{i + 1}) \in \mathbb{N} ^ i$ such that $f_i(\textbf{x}_2) = f_i(n_2, n_3, ..., n_{i + 1}) = \textbf{y}_2$, so $n_2, n_3, ..., n_{i + 1}$ exist\\
since $n_1, n_2, ..., n_{i + 1}$ exist, $\text{it is shown that }\forall \textbf{y} \in \mathbb{N} ^ 2, \exists \textbf{x} \in \mathbb{N} ^ 3, f(\textbf{x}) = \textbf{y}$\\
so $f_{i + 1}$ is surjective\\
\\
\\
\\
4.\\
(a)\\
need to show $f(C \cup D) \subset f(C) \cup f(D)$ and $f(C) \cup f(D) \subset f(C \cup D)$\\
\\
show $f(C \cup D) \subset f(C) \cup f(D)$\\
let $y \in f(C \cup D)$, then $\exists x \in C \cup D$ such that $f(x) = y$,\\
then $x \in C$ or $x \in D$,\\
then $f(x) \in f(C)$ or $f(x) \in f(D)$,\\
then $f(x) \in f(C) \cup f(D)$\\
\\
show $f(C) \cup f(D) \subset f(C \cup D)$\\
let $y \in f(C) \cup f(D)$,\\
then $y \in f(C)$ or $y \in f(D)$,\\
then $\forall y \in f(C), \exists x \in C$ such that $f(x) = y$\\
then $\forall y \in f(D), \exists x \in D$ such that $f(x) = y$\\
then $x \in C$ or $x \in D$,\\
then $\exists x \in C \cup D$ such that $f(x) = y$,\\
\\
(b)\\
$f(C \cup D) \subset f(C) \cap f(D)$\\
let $y \in f(C \cap D)$, then $\exists x \in C \cap D$ such that $f(x) = y$,\\
then $x \in C$ and $x \in D$,\\
then $f(x) \in f(C)$ and $f(x) \in f(D)$,\\
then $f(x) \in f(C) \cap f(D)$\\
\\
a function that $f: A \rightarrow B$. $C, D \subset A, f(C \cap D) \not\supset f(C) \cap f(D)$\\
let $A = \{0, 1, \frac{1}{2}\}, B = \{0, 1\}\\
C = \{0, 1\}, D = \{0, \frac{1}{2}\}$ and $f(0) = 0, f(1) = 1, f(\frac{1}{2}) = 1$,\\
then $C \cap D = \{0\},\\
f(C \cap D) = f(\{0\}) = \{0\}$\\
then $f(C) = f(\{0, 1\}) = \{0, 1\}\\
f(D) = f(\{0, \frac{1}{2}\}) = \{0, 1\}\\
f(C) \cap f(D) = \{0, 1\} \cap \{0, 1\} = \{0, 1\}\\
f(C \cap D) = f(\{0\}) = \{0\} \not\supset \{0, 1\} = f(C) \cap f(D)$\\
\\
\\
\\
5.\\
part 1
\[\sup E = b\]
since $\forall x \in E = (-\infty, b), x < b$, so $b$ is an upper bound\\
for contradiction, assume $b$ is not the least upper bound, then there exist an upper bound $i \in (-\infty, b)$ such that $i < b$, however, if $i < b$, then $i$ is not a upper bound of $E$ since $\neg\forall x \in E, x \leq i$, or equivalently, $\exists x \in (i, b) \subset E, x > i$, so the assumption that $b$ is not the least upper bound is wrong, so $b$ is the least upper bound\\
assume $\exists \varepsilon \in \mathbb{R}, \varepsilon > 0$ such that $b - \varepsilon < b$ is another upper bound lower than $b$, then
\begin{align*}
2b - \varepsilon &< 2b\\
\because (2b - \varepsilon) / 2 &< b\\
b - \varepsilon / 2 &< b\\ 
\therefore b - \varepsilon / 2 &\in E\\
\text{however, } b - \varepsilon / 2 &> b - \varepsilon
\end{align*}
$\because$ there exists an element in $E$ greater than $b - \varepsilon, \;\therefore b - \varepsilon$ is not an upper bound, which contradicts with the assumption that $b - \varepsilon$ is an upper bound, so $\neg\exists$ upper bound lower than $b$, so $b$ is least upper bound\\
\\
part 2\\
$E$ is unbounded below\\
for contradiction, assume $i \in E = (-\infty, b)$ is a lower bound\\
however, we can find a number $j \in E = (-\infty, i)$ such that $j < i$, then $i$ is not a lower bound of $E$ since $\neg\forall x \in E, x \geq i$, or equivalently, $\exists \varepsilon \in \mathbb{R}, \exists x = i - \varepsilon \in (-\infty, i) \subset E, x < i$, so the assumption that $b$ is a lower bound is wrong, so $b$ is not a lower bound\\
\\
\\
\\
6.\\
show $\inf B \leq \inf A$\\
$\forall a \in A, \because A \subset B, \therefore a \in B$, based on definition of $\inf B, \forall b \in B, \inf B \leq b$,\\
and since $a \in B, \therefore \inf B \leq a$\\
so $\inf B$ is a lower bound of $A$\\
$\inf A$ is greatest lower bound of $A$, so $\inf B \leq \inf A$\\
\\
show $\inf A \leq \sup A$\\
\begin{align*}
\inf A &= \sup(\{x : x \leq b, \forall b \in A\})\\
\sup A &= \inf(\{x: x \geq b, \forall b \in A\})\\
\end{align*}
since $lb := \inf A$ is a lower bound, $\forall x \in A, x \geq lb$\\
since $ub := \sup A$ is an upper bound, $\forall x \in A, x \leq ub$\\
so $\exists x \in A, lb \leq x \leq ub$\\
so $\inf A = lb \leq ub = \sup A$\\
\\
show $\sup A \leq \sup B$\\
$\forall a \in A, \because A \subset B, \therefore a \in B$, based on definition of $\sup B, \forall b \in B, \sup B \geq b$,\\
and since $a \in B, \therefore \sup B \geq a$\\
so $\sup B$ is an upper bound of $A$\\
$\sup A$ is least upper bound of $A$, so $\sup A \leq \sup B$
\\
\newpage
\noindent
7.\\
(a)\\
$c, c' \in B$\\
since $c = \sup B$, then
\[c = \inf(\{x: x \geq b, \forall b \in B\})\]
so $c \geq c'$\\
since $c' = \sup B$, then
\[c' = \inf(\{x: x \geq b, \forall b \in B\})\]
so $c' \geq c$\\
since $c \geq c'$ and $c' \geq c$, so $c = c'$\\
\\
\\
(b)\\
prove contraposition: if $x \in B$, then $x \leq c$\\
since $c$ is an upper bound of $B$, based on the definition of upper bound, $\forall x \in B, x \leq c$\\
\\
\\
8\\
(a)\\
assume $\exists \varepsilon > 0, \forall x \in B, x \leq c - \varepsilon, \text{ then } c - \varepsilon$ is an upper bound of $B$, then since $\sup B$ is a least upper bound, so $\sup B \leq c - \varepsilon$. since $\sup B \leq c - \varepsilon, \sup B \not= c$, so the assumption that $\forall x \in B, x \leq c - \varepsilon$ is wrong, so $\neg\forall x \in B, x \leq c - \varepsilon$, so $\exists x \in B, c - \varepsilon < x$. also, based on definition of $c = \sup B, \forall b \in B, b \leq c, $ so $x \leq c$\\
\\
(b)\\
need to prove $\forall \varepsilon > 0, \exists i \in B$ such that $d \leq i < d + \varepsilon$\\
since $d = \inf B$, d is a lower bound of B, so $\forall i < d, i \not\in B$\\
for contradiction, assume $[d, d + \varepsilon) \cap B$ is empty, then $\exists \varepsilon > 0, d \leq i < d + \varepsilon \longrightarrow i \not\in B$\\
contraposition is $i \in B \longrightarrow (i < d) \vee (i \geq d + \varepsilon)$\\
if $i < d = \inf B$, then since $d$ is a lower bound, $\forall b \in B, d \leq b$, since $i$ is smaller than a lower bound of $B$, this implies $i \not\in B$, but this contradicts with $i \in B$\\
if $i \geq d + \varepsilon$, then $d + \varepsilon$ is a lower bound of $B$, but $\inf B = d$, this contradicts with $d$ is a "greatest" lower bound\\
so the assumption that $[d, d + \varepsilon) \cap B$ is empty is wrong, so $[d, d + \varepsilon) \cap B$ is non-empty
\end{document}
