\documentclass[12pt, border = 4pt, multi]{article} % \documentclass[tikz, border = 4pt, multi]{article}
\usepackage[a4paper, margin = 70pt]{geometry}
\usepackage{lingmacros}
\usepackage{tree-dvips}
\usepackage{amssymb} % mathbb{}
\usepackage[dvipsnames]{xcolor}
\usepackage{forest}
\usepackage[pdftex]{hyperref}
\usepackage{amsmath} % matrices
\usepackage{xeCJK}
\usepackage{tikz}
\usepackage[arrowdel]{physics}
\usepackage{graphicx}
\usepackage{wrapfig}
\usepackage{listings}
\usepackage{pgfplots, pgfplotstable}
\usepackage{diagbox} % diagonal line in cell
\usepackage[usestackEOL]{stackengine}
\usepackage{makecell}
\usepackage{multirow}
\usepackage{multicol}
\usepackage[T1]{fontenc} 
\setlength{\columnsep}{1cm}
\graphicspath{{./img}} % specify the graphics path to be relative to the main .tex file, denoting the main .tex file directory as ./
\definecolor{orchid}{rgb}{0.7, 0.4, 1.1}
\lstset
{ 
  backgroundcolor = \color{white},
  basicstyle = \scriptsize,
  breaklines = true,
  commentstyle = \color{comment_color}\textit,
  keywordstyle = \color{keyword_color}\bfseries,
  language = c++,
  escapeinside = {\%*}{*)},          
  extendedchars = true,              
  frame = tb,
  numberstyle = \tiny\color{comment_color},
  rulecolor = \color{black},
  showstringspaces = false,
  stringstyle = \color{string_color},
  upquote = true, 
}
\usepackage{xcolor}
\definecolor{comment_color}{rgb}{0, 0.5, 0}
\definecolor{keyword_color}{rgb}{0.3, 0, 0.6}
\definecolor{string_color}{rgb}{0.5, 0, 0.1}
\begin{document}
\section*{Xi Liu}
collaboration: Chuanyang Jin\\
\\
1\\
definition 3.1.14, let $f: S \rightarrow \mathbb{R}$ be a function, $A \subset S$, $f|_A: A \rightarrow \mathbb{R}\\
f|_A(x) := f(x) \quad \forall x \in A$\\
definition 3.2.1, let $S \subset \mathbb{R}, c \in S, f: S \rightarrow \mathbb{R}$ be a function, $f$ is continuous at $c$ if $\forall \varepsilon > 0, \exists \delta > 0(x \in S \wedge |x - c| < \delta \rightarrow |f(x) - f(c)| < \varepsilon)$\\
\\
(a)\\
suppose $f: S \rightarrow \mathbb{R}$ is continuous at $c$, $\forall \varepsilon > 0, \exists \delta > 0(x \in S \wedge |x - c| < \delta \rightarrow |f(x) - f(c)| < \varepsilon)$\\
since $A \subset S, \forall x(x \in A \rightarrow x \in S)$\\
$f|_A: A \rightarrow \mathbb{R}, \forall \varepsilon > 0, \exists \delta > 0(x \in A \wedge |x - c| < \delta \rightarrow x \in S \wedge |x - c| \rightarrow |f|_A(x) - f(c)| < \varepsilon)$\\
\\
\\
\\
(b)\\
let $f: \mathbb{R} \rightarrow \mathbb{R}$ be a function\\
$f(x) :=
\begin{cases}
0 & \text{if } x \not= 0\\
1 & \text{if } x = 0\\
\end{cases}$\\
let $A := \{0\}$, then $f|_A$ is continuous at $c = 0 \in A$, since $\forall \varepsilon > 0, \exists \delta > 0(x \in A \wedge |x - c| < \delta \rightarrow |f(x) - f(c)| = |f(0) - f(0)| = 1 - 1 = 0 < \varepsilon)$, but $f$ is not continuous at $c$\\
\\
\\
\\
(c)\\
if $f|_A$ is continuous at $c$\\
$\forall \varepsilon > 0, \exists \delta > 0(x \in A = (c - \alpha, c + \alpha) \wedge |x - c| < \delta \rightarrow |f|_A(x) - f(c)| < \varepsilon)\\
A \subset S, \forall x(x \in A \rightarrow x \in S)\\
S \cap (c - \alpha, c)) \cup (S \cap (c, c + \alpha) = S \setminus \{c\}\\
\forall \varepsilon > 0, \exists \delta > 0(x \in S \wedge |x - c| < \delta \rightarrow |f(x) - f(c)| < \varepsilon)\\$
then $f$ is continuous at $c$\\
\newpage
\noindent
2\\
extreme value theorem 3.3.2, a continuous function $f: [a, b] \rightarrow \mathbb{R}$ on a closed and bounded interval $[a, b]$ achieves both an absolute minimum and an absolute maximum on $[a, b]$\\
intermediate value theorem 3.3.8, let $f: [a, b] \rightarrow \mathbb{R}$ be a continuous function. suppose $y \in \mathbb{R}$, $f(a) < y < f(b)$ or $f(b) < y < f(a)$, then $\exists c \in (a, b), f(c) = y$\\
\\
if $f: [a, b] \rightarrow \mathbb{R}$ is continuous, by extreme value theorem 3.3.2, $f$ achieves both an absolute minimum and an absolute maximum on $[a, b]$\\ $\min\{f([a, b])\} := f(x_1) := y_1\\
\max\{f([a, b])\} := f(x_2) := y_2$\\
so $f([a, b]) \subset [y_1, y_2]$\\
if $x_1 < x_2$, then by intermediate value theorem 3.3.8, if $y \in \mathbb{R}, f(x_1) < y < f(x_2)$, then $\exists c \in (x_1, x_2), f(c) = y$\\
so $f([a, b]) = [y_1, y_2]$, then $f([a, b])$ is a closed and bounded interval\\
if $x_1 = x_2$, then $f([a, b]) = \{f(x_1)\} = \{f(x_2)\}$, then $f([a, b])$ is a single number\\
so $f([a, b])$ is either a closed and bounded interval or single number\\
\\
\\
\\
3\\
(a)\\
part 1\\
proposition $P(n)$: $f$ is strictly increasing $\forall n \in \mathbb{N}$\\
base step: $n = 1$, $\forall x, y \in [0, \infty), x < y, \text{ then } f(x) = x ^ 1 < y ^ 1 = f(y)$\\
inductive step: assume $P(n)$ is true, then $x ^ n < y ^ n$\\
$x \cdot x ^ n < y \cdot y ^ n\\
x ^ {n + 1} < y ^ {n + 1}\\
f(x) < f(y)$\\
so $P(n + 1)$ is true\\
so $f$ is strictly increasing $\forall n \in \mathbb{N}$\\
\\
part 2\\
$\forall x, y \in [0, \infty)$, if $x \not= y$, then there are 2 cases\\
case 1: $x < y$, since $f$ is strictly increasing, $f(x) < f(y)$, so $f(x) \not= f(y)$\\
case 2: $y < x$, since $f$ is strictly increasing, $f(y) < f(x)$, so $f(x) \not= f(y)$\\
so $f$ is injective\\
\\
\\
\\
(b)\\
part 1\\
show $f$ is continuous $\forall n \in \mathbb{N}$\\
base step:\\
since $g_1(x) := x$ is continuous, by proposition 3.2.5 (iii), $g_1(x)g_1(x) = x ^ 2$ is also continuous\\
inductive step:\\
assume $g_n(x) := x ^ n$ is continuous, by proposition 3.2.5 (iii), $g_n(x)g_1(x) = x ^ n x = x ^ {n + 1}$ is also continuous\\
so $f$ is continuous $\forall n \in \mathbb{N}$\\
\\
part 2\\
show $f|_{[0, M]}: [0, M] \rightarrow [0, M ^ n]$ is surjective\\
show $\forall a \in [0, M ^ n], \exists x ^ n = a$, by intermediate value theorem 3.3.8, $\forall a \in [0, M ^ n], \exists c \in [0, M], f(c) = c ^ n = a$, so $f$ is surjective\\
$f$ is injective is shown in 3 (a) part 2\\
so $f$ is bijective\\
\\
\\
\\
(c)\\
assume $x$ is not unique, then $\exists x_1, x_2 \in \mathbb{R}, x_1 \not= x_2, f(x_1) = x_1 ^ n = f(x_2) = x_2 ^ n = a$\\
assume $x_1 < x_2$, since $f$ is strictly increasing, $f(x_1) < f(x_2), x_1 ^ n < x_2 ^ n\\
x_1 ^ n - x_2 ^ n > 0\\
a - a = 0 > 0$ is a contradiction\\
so the assumption that $x$ is not unique is false, so $x$ is unique\\
\\
\\
\\
\\
4
\begin{align*}
&\text{suppose } g \text{ is a monic polynomial of even degree } d\\
g(x) &= x ^ d + b_{d - 1} x ^ {d - 1} + ... + b_1 x + b_0\\
&\text{show } g(n) \text{ is positive}\\
&\text{compare highest order term with other terms}\\
\left|\frac{b_{d - 1} n ^ {d - 1} + ... + b_1 n + b_0}{n ^ d}\right|
&= \frac{|b_{d - 1} n ^ {d - 1} + ... + b_1 n + b_0|}{n ^ d}\\
&\leq \frac{|b_{d - 1}| n ^ {d - 1} + ... + |b_1| n + |b_0|}{n ^ d}\\
&\leq \frac{|b_{d - 1}| n ^ {d - 1} + ... + |b_1| n ^ {d - 1} + |b_0| n ^ {d - 1}}{n ^ d}\\
&= \frac{n ^ {d - 1}(|b_{d - 1}| + ... + |b_1| + |b_0|)}{n ^ d}\\
&= \frac{1}{n}(|b_{d - 1}| + ... + |b_1| + |b_0|)\\
\therefore \lim_{n \rightarrow \infty}\frac{b_{d - 1} n ^ {d - 1} + ... + b_1 n + b_0}{n ^ d} &= 0\\
\therefore \exists M \in \mathbb{N}, \left|\frac{b_{d - 1} M ^ {d - 1} + ... + b_1 M + b_0}{M ^ d}\right| &< 1\\
-(b_{d - 1} M ^ {d - 1} + ... + b_1 M + b_0) &< M ^ d\\
0 &< M ^ d + b_{d - 1} M ^ {d - 1} + ... + b_1 M + b_0 = g(M)
\end{align*}
so $g(M) > 0$, since $g(0) < 0$, by intermediate value theorem 3.3.8, $\exists c_1 \in (0, M), g(c_1) = 0$\\
$\lim_{x \rightarrow \infty} g(x) = \infty, \exists -M_2 < 0, g(-M_2) > 0$, by intermediate value theorem 3.3.8, $\exists c_2 \in (-M_2, 0), g(c_2) = 0$\\
\newpage
\noindent
5
\begin{align*}
\text{assume }\exists x_0, f(x_0) &\not= g(x_0)\\
\text{assume }f(x_0) &> g(x_0)\\
\Delta := |f(x_0) - g(x_0)| &> 0\\
\text{since }f, g&\text{ are continuous, then}\\
\forall \varepsilon > 0, &\exists \delta_1, \delta_2 > 0\\
|f(x_0) - f(x)| &< \varepsilon, \forall x \in S, |x - x_0| < \delta_1\\
|g(x) - g(x_0)| &< \varepsilon, \forall x \in S, |x - x_0| < \delta_2\\
\text{take } x \in E&\\
\Delta = |f(x_0) - g(x_0)| &= |f(x_0) - f(x) + g(x) - g(x_0)| \quad \text{(since } f(x) = g(x))\\
&\leq |f(x_0) - f(x)| + |g(x) - g(x_0)|
\end{align*}
which is false since $\varepsilon$ can be arbitrarily small, but $\Delta$ is a constant, so the assumption that $\exists x_0, f(x_0) \not= g(x_0)$ is false, so $\forall x \in S, f(x) = g(x)$\\
\\
\\
\\
\\
6
\begin{align*}
h(x) &= \alpha f(x) + \beta g(x)\\
\frac{h(x) - h(c)}{x - c} &= \frac{\alpha f(x) + \beta g(x) - (\alpha f(c) + \beta g(c))}{x - c}\\
&= \frac{\alpha f(x) - \alpha f(c)}{x - c} + \frac{\beta g(x) - \beta g(c)}{x - c}\\
&= \alpha\frac{f(x) - f(c)}{x - c} + \beta\frac{g(x) - g(c)}{x - c}\\
&\text{by corollary 3.1.12}\\
h'(c) = \lim_{x \rightarrow c}\frac{h(x) - h(c)}{x - c} &= \alpha\lim_{x \rightarrow c}\frac{f(x) - f(c)}{x - c} + \beta\lim_{x \rightarrow c}\frac{g(x) - g(c)}{x - c}\\
&= \alpha f'(c) + \beta g'(c)\\
\end{align*}
\\
\\
\\
\\
7
\begin{align*}
h(x) &= f(x) g(x)\\
\frac{h(x) - h(c)}{x - c} &= \frac{f(x)g(x) - f(c)g(c)}{x - c}\\
&= \frac{f(x)g(x) - f(x)g(c) + f(x)g(c) - f(c)g(c)}{x - c}\\
&= \frac{f(x)(g(x) - g(c)) + (f(x) - f(c))g(c)}{x - c}\\
&= f(x)\frac{g(x) - g(c)}{x - c} + g(c)\frac{f(x) - f(c)}{x - c}\\
&\text{by corollary 3.1.12}\\
h'(c) &= \left(\lim_{x \rightarrow c}f(x)\right)\left(\lim_{x \rightarrow c}\frac{g(x) - g(c)}{x - c}\right) + \left(\lim_{x \rightarrow c}(g(c)\right)\left(\lim_{x \rightarrow c}\frac{f(x) - f(c)}{x - c}\right)\\
&= f(c)g'(c) + g(c)f'(c)\\
&= f(c)g'(c) + f'(c)g(c)\\
\end{align*}
\\
\\
\\
\\
8
\begin{align*}
x > 0, c > 0, x &\not= c\\
f(x) &= \sqrt{x}\\
\frac{\sqrt{x} - \sqrt{c}}{x - c} &= \frac{\sqrt{x} - \sqrt{c}}{(\sqrt{x} - \sqrt{c})(\sqrt{x} + \sqrt{c})}\\
&= \frac{1}{\sqrt{x} + \sqrt{c}}\\
f'(c) &= \lim_{x \rightarrow c}\frac{\sqrt{x} - \sqrt{c}}{x - c}\\
&= \lim_{x \rightarrow c}\frac{1}{\sqrt{x} + \sqrt{c}}\\
&= \frac{1}{2\sqrt{c}}
\end{align*}
so $f(x) = \sqrt{x}$ is differentiable at all $c \in (0, \infty)$\\
\end{document}
