\documentclass[12pt, border = 4pt, multi]{article} % \documentclass[tikz, border = 4pt, multi]{article}
\usepackage[a4paper, margin = 70pt]{geometry}
\usepackage{lingmacros}
\usepackage{tree-dvips}
\usepackage{amssymb} % mathbb{}
\usepackage[dvipsnames]{xcolor}
\usepackage{forest}
\usepackage[pdftex]{hyperref}
\usepackage{amsmath} % matrices
\usepackage{xeCJK}
\usepackage{tikz}
\usepackage[arrowdel]{physics}
\usepackage{graphicx}
\usepackage{wrapfig}
\usepackage{listings}
\usepackage{pgfplots, pgfplotstable}
\usepackage{diagbox} % diagonal line in cell
\usepackage[usestackEOL]{stackengine}
\usepackage{makecell}
\usepackage{mathrsfs}
\usepackage{multirow}
\usepackage{multicol}
\usepackage[T1]{fontenc}
\allowdisplaybreaks[1]
\setlength{\columnsep}{1cm}
\graphicspath{{./img}} % specify the graphics path to be relative to the main .tex file, denoting the main .tex file directory as ./
\definecolor{orchid}{rgb}{0.7, 0.4, 1.1}
\lstset
{ 
  backgroundcolor = \color{white},
  basicstyle = \scriptsize,
  breaklines = true,
  commentstyle = \color{comment_color}\textit,
  keywordstyle = \color{keyword_color}\bfseries,
  language = c++,
  escapeinside = {\%*}{*)},          
  extendedchars = true,              
  frame = tb,
  numberstyle = \tiny\color{comment_color},
  rulecolor = \color{black},
  showstringspaces = false,
  stringstyle = \color{string_color},
  upquote = true, 
}
\usepackage{xcolor}
\definecolor{comment_color}{rgb}{0, 0.5, 0}
\definecolor{keyword_color}{rgb}{0.3, 0, 0.6}
\definecolor{string_color}{rgb}{0.5, 0, 0.1}
\begin{document}
\section*{Xi Liu}
1\\
(a)\\
definition 3.5.1\\
for $f(x)$ to converge to $L$ as $x \rightarrow -\infty$\\
$\forall \varepsilon > 0, \exists M \in \mathbb{R}, \forall x \leq M, |f(x) - L| < \varepsilon$\\
\\
\\
\begin{align*}
\lim_{x \rightarrow \infty} \frac{1}{1 + x ^ 2} &= 0\\
\left|\frac{1}{1 + x ^ 2} - 0\right| &< \varepsilon\\
\frac{1}{1 + x ^ 2} &< \varepsilon\\
1 + x ^ 2 &> \frac{1}{\varepsilon}\\
x ^ 2 &> \frac{1}{\varepsilon} - 1\\
x &> \sqrt{\frac{1}{\varepsilon} - 1}\\
\forall \varepsilon > 0, \exists M := \sqrt{\frac{1}{\varepsilon} - 1} \in \mathbb{R}, &\forall x \geq M = \sqrt{\frac{1}{\varepsilon} - 1}\\
|f(x) - L| &= \left|\frac{1}{1 + x ^ 2} - 0\right| < \varepsilon
\end{align*}
\begin{align*}
\lim_{x \rightarrow -\infty} \frac{1}{1 + x ^ 2} &= 0\\
\left|\frac{1}{1 + x ^ 2} - 0\right| &< \varepsilon\\
\frac{1}{1 + x ^ 2} &< \varepsilon\\
1 + x ^ 2 &> \frac{1}{\varepsilon}\\
x ^ 2 &> \frac{1}{\varepsilon} - 1\\
x &< -\sqrt{\frac{1}{\varepsilon} - 1}\\
\forall \varepsilon > 0, \exists M := -\sqrt{\frac{1}{\varepsilon} - 1} \in \mathbb{R}, &\forall x \leq M = -\sqrt{\frac{1}{\varepsilon} - 1}\\
|f(x) - L| = \left|\frac{1}{1 + x ^ 2} - 0\right| < \varepsilon\\
\end{align*}
\\
\\
\\
(b)\\
definition 3.2.1, $S \subset \mathbb{R}, c \in S, f: S \rightarrow \mathbb{R}$ is continuous at $c$ if\\
$\forall \varepsilon > 0, \exists \delta > 0, (x \in S \wedge |x - c| < \delta \rightarrow |f(x) - f(c)| < \varepsilon)$\\
\\
since $\lim_{x \rightarrow \infty} f(x) = L\\
\forall \varepsilon > 0, \exists M \in \mathbb{R}, \forall x \geq M, |f(x) - L| < \varepsilon\\$
\\
since $\lim_{x \rightarrow -\infty} f(x) = L\\
\forall \varepsilon > 0, \exists M \in \mathbb{R}, \forall x \leq M, |f(x) - L| < \varepsilon$\\
\\
need to show $\forall \varepsilon > 0, \exists \delta > 0, (y \in S \wedge |y - 0| < \delta \rightarrow |g(y) - g(0)| < \varepsilon)\\
\textcircled{1} \because \lim_{x \rightarrow \infty} f(x) = L, \exists M_0 \in \mathbb{R}, \forall 1 / y \geq M_0, |f(1 / y) - L| < \varepsilon\\
\textcircled{2} \because \lim_{x \rightarrow -\infty} f(x) = L, \exists M_1 \in \mathbb{R}, \forall 1 / y \leq M_1, |f(1 / y) - L| < \varepsilon\\
\textcircled{1}, \text{if } y > 0, 1 / y \geq M_0, 0 < y \leq 1 / M_0\\
\textcircled{2}, \text{if } y < 0, 1 / y \leq M_1, 0 > y \geq 1 / M_1\\
\textcircled{3}, \text{if } y = 0, |g(y) - g(0)| = |L - L| = 0 <  \varepsilon\\
\text{combine }\textcircled{1}, \textcircled{2}, 1 / M_1 \leq y \leq 1 / M_0\\
\text{let } M := \max\{|M_0|, |M_1|\}\\
-1 / M \leq y \leq 1 / M\\
|y| \leq 1 / M\\
\therefore \exists \delta := 1 / M\\
|y - 0| < \delta = 1 / M \rightarrow |g(y) - g(0)| = |f(1 / y) - L| < \varepsilon$\\
\\
\\
\\
(c)\\
if $f$ is continuous at 0\\
$\forall \varepsilon > 0, \exists \delta > 0, (x \in S \wedge |x - 0| < \delta \rightarrow |f(x) - f(0)| < \varepsilon)\\
1 / y \in S \wedge |1 / y - 0| < \delta \rightarrow |f(1 / y) - f(0)| < \varepsilon\\
|1 / y - 0| < \delta\\
|1 / y| < \delta\\
-\delta < 1 / y < \delta\\
\textcircled{1}, -1 / \delta > y\\
\textcircled{2}, y > 1 / \delta\\$\\
\\
$\forall \varepsilon > 0, \exists M \in \mathbb{R}, \forall y \geq M := 1 / \delta, |g(y) - f(0)| = |f(1 / y) - f(0)| < \varepsilon\\
\therefore \lim_{y \rightarrow \infty} g(y) = f(0)$\\
\\
$\forall \varepsilon > 0, \exists M \in \mathbb{R}, \forall y \leq M := -1 / \delta, |g(y) - f(0)| = |f(1 / y) - f(0)| < \varepsilon\\
\therefore \lim_{y \rightarrow -\infty} g(y) = f(0)\\
\\
\therefore \lim_{y \rightarrow \infty} g(y) = \lim_{y \rightarrow -\infty} g(y) = f(0)$\\
\\
\\
\\
\\
2\\
(a)\\
part 1\\
let $\{x_n\}$ be a sequence satisfying $x_n \in [a, b], \forall n \in \mathbb{N}\\$
based on bolzano weierstrass theorem, since $\{x_n\}$ is bounded, there exists a convergent subsequence $\{x_{n_i}\}$, $\{x_{n_i}\}$ converge to a number $L \in \mathbb{R}$. since $\{x_{n_i}\}$ is a subsequence of $\{x_n\}$, $\{x_{n_i}\}$ is a sequence satisfying $x_{n_i} \in [a, b], \forall n \in \mathbb{N}$\\
\\
assume $[a, b]$ is not sequentially compact, then $L \not\in [a, b]$, then $L < a$ or $L > b$\\
if $L > b, L - b > 0$, since $\{x_{n_i}\}$ converges to $L, \forall \varepsilon > 0, \exists M \in \mathbb{N}, \forall n \geq M, |x_{n_i} - L| < \varepsilon$\\
take $\varepsilon < L - b\\
|x_{n_i} - L| < \varepsilon < L - b\\
|x_{n_i} - L| < L - b\\
b - L < x_{n_i} - L < L - b\\
b - L < x_{n_i} - L\\
b < x_{n_i}$\\
which contradicts with $x_{n_i} \in [a, b]$, so the assumption that $[a, b]$ is not sequentially compact is false, so $\{x_n\}$ is sequentially compact\\
\\
if $L < a, a - L > 0$, since $\{x_{n_i}\}$ converges to $L, \forall \varepsilon > 0, \exists M \in \mathbb{N}, \forall n \geq M, |x_{n_i} - L| < \varepsilon$\\
take $\varepsilon < a - L\\
|x_{n_i} - L| < \varepsilon < a - L\\
|x_{n_i} - L| < a - L\\
L - a < x_{n_i} - L < a - L\\
x_{n_i} - L < a - L\\
x_{n_i} < a$\\
which contradicts with $x_{n_i} \in [a, b]$, so the assumption that $[a, b]$ is not sequentially compact is false, so $[a, b]$ is sequentially compact\\
\\
\\
\\
part 2\\
{\large$\{x_n\} = \{b - \frac{1}{n}\}$} is a sequence satisfying $x_n \in K = (a, b)$ that converge to $b$ (since $\forall \varepsilon > 0, \exists M \in \mathbb{N}, 0 < 1 / M < \varepsilon, \forall n \geq M, |x_n - 0| = |1 / n| = 1 / n \leq 1 / M < \varepsilon$, and based on continuity of algebraic operations 2.2.2), since $x_n \in (a, b)$, so $\{x_n\}$ is bounded, based on proposition 2.3.7, since $\{x_n\}$ is bounded sequence that converge to $b$, so every convergent subsequence $\{x_{n_k}\}$ converges to $b$, but $b \not\in (a, b)$, so there does not exist a subsequence $\{x_{n_k}\}$ and point $x \in K$ such that $x_{n_k} \rightarrow x$ as $k \rightarrow \infty$, so $(a, b)$ is not sequentially compact\\
\\
\\
\\
(b)\\
contrapositive: if set $K$ is not bounded, then the set $K$ is not sequentially compact\\
for every sequence $x_n \in K$, since $K$ is unbounded, based on definition 1.3.6\\
$x_n \geq n, x_{n_k} > n_k > k$\\
/* show for any subsequence $\{x_n\}_{i = 1} ^ {\infty}, \forall i \in \mathbb{N}, n_i \geq i$\\
base step: $i = 1, 1 \leq n_1, \because n_1 \in \mathbb{N}$\\
inductive step: assume $i \leq n_i$ is true, show $i + 1 \leq n_{i + 1}$ is true
\begin{align*}
i &\leq n_i\\
i + 1 &\leq n_i + 1\\
&\leq n_{i + 1}
\end{align*}
$\because n_i, n_{i + 1} \in \mathbb{N}, n_i < n_{i + 1}$ implies $n_i \not= n_{i + 1}\\
\text{least possible } n_{i + 1} \text{ is } n_i + 1\;\therefore n_i + 1 \leq n_{i + 1}$ */\\
$\because x_{n_k} > k$, every subsequence $\{x_{n_k}\}$ diverges, so there is no subsequence $\{x_{n_k}\}$ and point $x \in K$ such that $x_{n_k} \rightarrow x$ as $k \rightarrow \infty$, so $K \subset \mathbb{R}$ is not sequentially compact\\
\\
\\
\\
(c)\\
let $s := \sup(K)\\
\text{since } \mathbb{Q} \text{ is dense in } \mathbb{R}\\
\exists x_n \in (s - 1 / n, s)\\
s - 1 / n < x_n < s\\
\because \lim_{n \rightarrow \infty} s - 1 / n = s\\
\lim_{n \rightarrow \infty} s = s\\
\text{based on squeeze lemma 2.2.1}\\
\lim_{n \rightarrow \infty} \{x_n\} = s\\$
based on proposition 2.3.7, since $\{x_n\}$ is a bounded sequence that converge to $s$, every convergent subsequence $\{x_{n_k}\}$ converges to $s$, since $K$ is sequentially compact, so every sequence in $K$ has a convergent subsequence converging to a point in $K$, so $s$ is a point in $K$, $s = \sup K \in K$\\
\\
\\
\\
let $i := \inf(K)\\
\text{since } \mathbb{Q} \text{ is dense in } \mathbb{R}\\
\exists x_n \in (i, i + 1 / n)\\
i < x_n < i + 1 / n\\
\because \lim_{n \rightarrow \infty} i = i\\
\lim_{n \rightarrow \infty} i + 1 / n = i\\
\text{based on squeeze lemma 2.2.1}\\
\lim_{n \rightarrow \infty} \{x_n\} = i\\$
based on proposition 2.3.7, since $\{x_n\}$ is a bounded sequence that converge to $i$, every convergent subsequence $\{x_{n_k}\}$ converges to $i$, since $K$ is sequentially compact, so every sequence in $K$ has a convergent subsequence converging to a point in $K$, so $i$ is a point in $K$, $i = \inf K \in K$\\
\\
\\
\\
(d)\\
definition 3.2.1, $S \subset \mathbb{R}, c \in S, f: S \rightarrow \mathbb{R}$ is continuous at $c$ if\\
$\forall \varepsilon > 0, \exists \delta > 0, (x \in S \wedge |x - c| < \delta \rightarrow |f(x) - f(c)| < \varepsilon)$\\
definition 0.3.13, direct image $f: K \rightarrow \mathbb{R}$, direct image is $f(K) = \{f(x) \in \mathbb{R}: x \in K\}$\\
\\
part 1\\
show every sequence in $f(K)$ has a convergent subsequence converging to a point in $f(K)$\\
pick a sequence $\{y_n\} \subset f(K)$, $y_n \in f(K)$, so $y_n = f(x_n)$ for some $x_n \in K$\\
\\
since $K$ is sequentially compact, $\{x_n\}$ has a subsequence $\{x_{n_k}\}$ and a point $x \in K$ such that $x_{n_k} \rightarrow x \in K$ as $k \rightarrow \infty$, bolzano weierstrass theorem 2.3.3\\
\\
since $f$ is continuous
\[y = \lim_{k \rightarrow \infty} y_{n_k} = \lim_{k \rightarrow \infty} f(x_{n_k}) = f(x)\]
$f(x_{n_k}) \rightarrow f(x) \in f(K), y \in f(K)$, so $f(K)$ is closed\\
\\
for contradiction, assume $f(K)$ is not bounded\\
suppose there is a sequence $\{b_n\} \subset f(K)$ with $\forall n \in \mathbb{N}, n \leq b_n$\\
suppose there is a sequence $\{a_n\} \subset K$ with $f(a_n) = b_n, \{a_n\}$ is contained in $K$ so have a subsequence $a_{n_k}$ converging to some $a \in K$, but since $f(a) \in \mathbb{R}$
\[\lim_{k \rightarrow \infty} n_k \leq \lim_{k \rightarrow \infty} f(a_{n_k}) = f(a)\]
which is a contradiction, so $f(K)$ is bounded\\
$f(x_{n_k})$ is a subsequence of $\{y_n\}$\\
so $f(K)$ is sequentially compact\\
\\
\\
part 2\\
based on what is shown in problem 2.(a), $[a, b]$ is sequentially compact, so $K$ is a closed and bounded interval\\
since $f$ is a continuous function on a closed and bounded interval $K$, based on extreme value (min max) theorem 3.3.2, $f$ achieves both an absolute minimum and an absolute maximum on $K$\\
\\
\\
\\
3\\
(a)\\
let $x_0, c, x \in [a, b], x_0 < c < x$\\
use taylor's theorem at $x$, with $n = 0$\\
$f(x) = P_0 ^ {x_0}(x) + f'(c)(x - x_0) = f(x_0) + f'(c)(x - x_0)\\$
replace $x$ with $x + h$, replace $x_0$ with $x$\\
$f(x + h) = f(x) + f'(c)(x + h - x) = f(x) + f'(c)h$
\begin{align*}
\frac{f(x + h) - f(x)}{h} &= f'(c)\\
\text{let } c &\in [x, x + h]\\
&\text{based on mean value theorem 4.2.3}\\
|f'(c) - f'(x)| &= |f''(d)(c - x)| \leq |f''(d)|h\\
&\text{take } M := \max\{|f''(d)|\}, d \in [x, x + h]\\
M_1 &= -M,\quad M_2 = M\\
M_1 &\leq |f'(c) - f'(x)| \leq M_2\\
\end{align*}
\\
\\
\\
(b)\\
let $x_0, c, x \in [a, b], x_0 < c < x$\\
use taylor's theorem at $x$, with $n = 2$
\begin{align*}
\textcircled{1}, f(x) &= P_2 ^ {x_0}(x) + f ^ {(3)}(c)(x - x_0)\\
&= f(x_0) + f'(x_0)(x - x_0) + \frac{f''(x_0)}{2!}(x - x_0) ^ 2 + \frac{f ^ {(3)}(c)}{3!}(x - x_0) ^ 3\\
&\text{from }\textcircled{1}, \text{replace $x$ with $x + h$, replace $x_0$ with $x$, replace $c$ with $c_1$}\\
f(x + h) &= f(x) + f'(x)(x + h - x) + \frac{f''(x)}{2}(x + h - x) ^ 2 + \frac{f ^ {(3)}(c_1)}{3!}(x + h - x) ^ 3\\
&= f(x) + f'(x)h + \frac{f''(x)}{2}h ^ 2 + \frac{f ^ {(3)}(c_1)}{3!}h ^ 3\\
&\text{from }\textcircled{1}, \text{replace $x$ with $x - h$, replace $x_0$ with $x$, replace $c$ with $c_2$}\\
f(x - h) &= f(x) + f'(x)(x - h - x) + \frac{f''(x)}{2}(x - h - x) ^ 2 + \frac{f ^ {(3)}(c_2)}{3!}(x - h - x) ^ 3\\
&= f(x) - f'(x)h + \frac{f''(x)}{2}h ^ 2 - \frac{f ^ {(3)}(c_2)}{3!} h ^ 3\\
\frac{f(x + h) - f(x - h)}{2h} &= \frac{2f'(x)h + \frac{f ^ {(3)}(c_1)}{3!}h ^ 3 - \frac{f ^ {(3)}(c_2)}{3!} h ^ 3}{2h}\\
&= \frac{2f'(x)h + \frac{1}{6}(f ^ {(3)}(c_1)h ^ 3 - f ^ {(3)}(c_2)h ^ 3)}{2h}\\
&= f'(x) + \frac{1}{12}(f ^ {(3)}(c_1)h ^ 2 - f ^ {(3)}(c_2)h ^ 2)\\
&= f'(x) + \frac{f ^ {(3)}(c_1) - f ^ {(3)}(c_2)}{12}h ^ 2\\
f'(x) - \frac{f(x + h) - f(x - h)}{2h} &= f'(x) - \left(f'(x) + \frac{f ^ {(3)}(c_1) - f ^ {(3)}(c_2)}{12}h ^ 2\right)\\
&= \frac{f ^ {(3)}(c_1) - f ^ {(3)}(c_2)}{12}h ^ 2\\
&\leq \frac{|f ^ {(3)}(c_1)| + |f ^ {(3)}(c_2)|}{12}h ^ 2\\
&\leq \frac{2 \max\{|f ^ {(3)}(c_1)|, |f ^ {(3)}(c_2)|\}}{12}h ^ 2\\
\text{take } M &:= \frac{2 \max\{|f ^ {(3)}(c_1)|, |f ^ {(3)}(c_2)|\}}{12}\\
M_3 = -M, &\quad M_4 = M\\
\end{align*}
\\
\\
\\
(c)\\
part 1\\
let $x_0, c, x \in [a, b], x_0 < c < x$\\
use taylor's theorem at $x$, with $n = 1$\\
\begin{align*}
\textcircled{1}, f(x) &= P_1 ^ {x_0}(x) + f''(c)(x - x_0)\\
&= f(x_0) + f'(x_0)(x - x_0) + \frac{f''(c)}{2!}(x - x_0) ^ 2\\
&\text{from }\textcircled{1}, \text{replace $x$ with $x + h$, replace $x_0$ with $x$, replace $c$ with $c_1$}\\
c_1 &\in [x, x + h]\\
f(x + h) &= f(x) + f'(x)(x + h - x) + \frac{f''(c_1)}{2!}(x + h - x) ^ 2\\
f(x + h) &= f(x) + f'(x)h + \frac{f''(c_1)}{2!}h ^ 2\\
-\frac{f''(c_1)}{2!}h ^ 2 &= f'(x)h - (f(x + h) - f(x))\\
\left|-\frac{f''(c_1)}{2!}h\right| &= \left|f'(x) - \frac{f(x + h) - f(x)}{h}\right|\\
\left|\frac{f''(c_1)}{2}h\right| &= \left|f'(x) - \frac{f(x + h) - f(x)}{h}\right|\\
\frac{h}{2}|f''(c_1)| &= \left|f'(x) - \frac{f(x + h) - f(x)}{h}\right|\\
\\
\left|f'(x) - \frac{f(x + h) - f(x)}{h}\right| &= \frac{h}{2}|f''(c_1)|\\
&= \frac{h}{2}|-k ^ 2\sin(kc_1)|\\
&\leq\frac{h}{2} k ^ 2\\
&= \frac{k ^ 2 h}{2}\\
\end{align*}
\\
\\
\\
part 2\\
from problem 3.(b)
\begin{align*}
f'(x) - \frac{f(x + h) - f(x - h)}{2h} &= \frac{f ^ {(3)}(c_1) - f ^ {(3)}(c_2)}{12}h ^ 2\\
\left|f'(x) - \frac{f(x + h) - f(x - h)}{2h}\right| &= \left|\frac{f ^ {(3)}(c_1) - f ^ {(3)}(c_2)}{12}h ^ 2\right|\\
&= \left|\frac{(-k ^ 3\cos(kc_1)) - (-k ^ 3\cos(kc_2))}{12}h ^ 2\right|\\
&= \left|\frac{-k ^ 3\cos(kc_1) + k ^ 3\cos(kc_2)}{12}h ^ 2\right|\\
&= \left|\frac{k ^ 3(\cos(kc_2) - \cos(kc_1))}{12}h ^ 2\right|\\
&= |\cos(kc_2) - \cos(kc_1)|\left|\frac{k ^ 3 h ^ 2}{12}\right|\\
&\leq ||\cos(kc_2)| + |\cos(kc_1)||\left|\frac{k ^ 3 h ^ 2}{12}\right|\\
&\leq \frac{2 k ^ 3 h ^ 2}{12}\\
&= \frac{k ^ 3 h ^ 2}{6}\\
\end{align*}
\\
\\
\\
4\\
(a)\\
\begin{align*}
m_i &= \inf\{f(x): x_{i - 1} \leq x \leq x_i\}\\
M_i &= \sup\{f(x): x_{i - 1} \leq x \leq x_i\}\\
L(\mathcal{P}, f) &= \sum_{i = 1} ^ n m_i \Delta x_i\\
U(\mathcal{P}, f) &= \sum_{i = 1} ^ n M_i \Delta x_i\\
\forall c_i &\in [x_{i - 1}, x_i]\\
\inf\{f(x): x_{i - 1} &\leq x \leq x_i\} \leq f(c_i) \leq \sup\{f(x): x_{i - 1} \leq x \leq x_i\}\\
\forall i \in \{1, 2, ..., n\}, m_i &\leq f(c_i) \leq M_i\\
\sum_{i = 1} ^ n m_i &\leq \sum_{i = 1} ^ n f(c_i) \leq \sum_{i = 1} ^ n M_i\\ 
\sum_{i = 1} ^ n m_i \Delta x_i &\leq \sum_{i = 1} ^ n f(c_i)\Delta x_i \leq \sum_{i = 1} ^ n M_i \Delta x_i\\
L(\mathcal{P}, f) &\leq \sum_{i = 1} ^ n f(c_i)\Delta x_i \leq U(\mathcal{P}, f)\\
\end{align*}
\\
\\
\\
(b)\\
definition 5.1.9, riemann integrable
\begin{align*}
\int_a ^ b f(x) dx &=  \underline{\int_a ^ b}f(x)dx = \overline{\int_a ^ b}f(x)dx\\
\underline{\int_a ^ b}f(x)dx &= \sup\{L(P, f): P \text{ a partition of }[a, b]\}\\
\overline{\int_a ^ b}f(x)dx &= \inf\{U(P, f): P \text{ a partition of }[a, b]\}\\
\\
\int_a ^ b f &= \underline{\int_a ^ b} f = \sup\{L(P, f)\}\\
\text{let } P_1 \text{ be a partition of }[a, b], \int_a ^ b f - \varepsilon &< L(P_1, f) < \underline{\int_a ^ b} f\\
\\
\int_a ^ b f &= \overline{\int_a ^ b} f = \inf\{U(P, f)\}\\
\text{let } P_2 \text{ be a partition of }[a, b], \overline{\int_a ^ b} f &< U(P_2, f) < \int_a ^ b f + \varepsilon\\
\\
\text{let } P_3 \text{ be a partition of }[a, b], P_3 := P_1 \cup P_2\\
\because P_1 \subset P_3, P_3 \text{ is a refinement of } P_1, &\therefore L(P_1, f) \leq L(P_3, f)\\
\because P_2 \subset P_3, P_3 \text{ is a refinement of } P_2, &\therefore U(P_3, f) \leq U(P_1, f)\\
\int_a ^ b f - \varepsilon < L(P_1, f) \leq L(P_3, f) \leq &\sum_{i = 1} ^ n f(x_i)\Delta x_i \leq U(P_3, f) \leq U(P_2, f) < \int_a ^ b f + \varepsilon\\
\int_a ^ b f - \varepsilon < &\sum_{i = 1} ^ n f(x_i)\Delta x_i < \int_a ^ b f + \varepsilon\\
- \varepsilon < &\sum_{i = 1} ^ n f(x_i)\Delta x_i - \int_a ^ b f < \varepsilon\\
\left|\sum_{i = 1} ^ n f(x_i)\Delta x_i - \int_a ^ b f\right| &< \varepsilon\\
\left|\int_a ^ b f - \sum_{i = 1} ^ n f(x_i)\Delta x_i\right| &< \varepsilon\\
\end{align*}
\\
\\
\\
(c)\\
part 1
\begin{align*}
R_n(f, [0, 1]) &= \sum_{i = 1} ^ n f(x_i) \Delta x\\
\Delta x &= \frac{b - a}{n} = \frac{1}{n}\\
x_i &= a + (b - a)(i / n) = 0 + (1 - 0)(i / n) = \frac{i}{n}\\
\because i / n \in \mathbb{Q}, f(i / n) = 1\\
R_n(f, [0, 1]) &= \sum_{i = 1} ^ n (1)(1 / n)\\
&= \sum_{i = 1} ^ n \frac{1}{n}\\
&= 1\\
\therefore \{R_n(f, [0, 1])\}_{n = 1} ^ {\infty} &= \{1\}_{n = 1} ^ {\infty} \text{ converges to 1}\\
\end{align*}
\\
\\
part 2
\begin{align*}
R_n(f, [1, 1 + \sqrt{2}]) &= \sum_{i = 1} ^ n f(x_i) \Delta x\\
\Delta x &= \frac{b - a}{n} = \frac{1 + \sqrt{2} - 1}{n} = \frac{\sqrt{2}}{n}\\
x_i &= a + (b - a)(i / n) = 1 + (1 + \sqrt{2} - 1)(i / n) = 1 + (\sqrt{2}i / n)\\
\because \sqrt{2}i / n \not\in \mathbb{Q}, 1 + (\sqrt{2}i / n) \not\in \mathbb{Q}, &f(1 + (\sqrt{2}i / n)) = 0\\
R_n(f, [1, 1 + \sqrt{2}]) &= \sum_{i = 1} ^ n 0 (\sqrt{2} / n)\\
&= 0\\
\therefore \{R_n(f, [0, 1])\}_{n = 1} ^ {\infty} &= \{0\}_{n = 1} ^ {\infty} \text{ converges to 0}\\
\end{align*}
\\
\\
part 3
\begin{align*}
R_n(f, [0, 1 + \sqrt{2}]) &= \sum_{i = 1} ^ n f(x_i) \Delta x\\
\Delta x &= \frac{b - a}{n} = \frac{1 + \sqrt{2} - 0}{n} = \frac{1 + \sqrt{2}}{n}\\
x_i &= a + (b - a)(i / n) = 0 + (1 + \sqrt{2} - 0)(i / n) = (1 + \sqrt{2})(i / n)\\
&= i / n + (\sqrt{2}i / n)\\
\because \sqrt{2}i / n \not\in \mathbb{Q}, i / n + (\sqrt{2}i / n) \not\in \mathbb{Q}, &f(i / n + (\sqrt{2}i / n)) = 0\\
R_n(f, [0, 1 + \sqrt{2}]) &= \sum_{i = 1} ^ n (0) \frac{1 + \sqrt{2}}{n}\\
&= 0\\
\therefore \{R_n(f, [0, 1 + \sqrt{2}])\}_{n = 1} ^ {\infty} &= \{0\}_{n = 1} ^ {\infty} \text{ converges to 0}\\
\end{align*}
\\
\\
part 4
\begin{align*}
R_n(f, [0, 1]) + R_n(f, [1, 1 + \sqrt{2}]) = 1 + 0 = 1 &\not= R_n(f, [0, 1 + \sqrt{2}]) = 0\\
\lim_{n \rightarrow \infty} R_n(f, [0, 1]) + R_n(f, [1, 1 + \sqrt{2}]) = 1 + 0 = 1 &\not= \lim_{n \rightarrow \infty}  R_n(f, [0, 1 + \sqrt{2}]) = 0\\
\end{align*}
\\
\\
\\
(d)\\
disprove\\
$\{R_n(f, [0, 1])\}$ converges to 1 as $n \rightarrow \infty$ as shown in 4.(c) part 1\\
but the dirichlet function defined in 4.(c) is not riemann integrable since
\begin{align*}
m_i &= \inf\{f(x): x_{i - 1} \leq x \leq x_i\} = 0\\
M_i &= \sup\{f(x): x_{i - 1} \leq x \leq x_i\} = 1\\
L(P, f) &= \sum_{i = 1} ^ n m_i \Delta x_i = \sum_{i = 1} ^ n (0)\Delta x_i = 0\\
U(P, f) &= \sum_{i = 1} ^ n M_i \Delta x_i = \sum_{i = 1} ^ n (1)\Delta x_i = \sum_{i = 1} ^ n \Delta x_i = 1 - 0 = 1\\
\underline{\int_a ^ b}f(x)dx &= \sup\{L(P, f): P \text{ a partition of }[a, b]\} = 0\\
\overline{\int_a ^ b}f(x)dx &= \inf\{U(P, f): P \text{ a partition of }[a, b]\} = 1\\
\underline{\int_a ^ b}f(x)dx &= 0 \not= \overline{\int_a ^ b}f(x)dx = 1
\end{align*}
so $f$ is not riemann integrable\\
\end{document}
